hardware/ag32VerilogScript.sml
@@ -1,11 +1,14 @@
 open hardwarePreamble;
 
-open alistTheory;
+open alignmentTheory alistTheory;
 
 open verilogTranslatorLib moduleTranslatorTheory;
 open verilogTranslatorConfigLib ag32MachineTheory ag32AddAcceleratorTheory ag32EqTheory;
 
 val _ = new_theory "ag32Verilog";
+
+guess_lengths ();
+prefer_num ();
 
 (*
 (* Based on Magnus' code from mail *)
@@ -124,40 +127,263 @@ val computer_Next_relM = Q.store_thm("computer_next_relM",
  impl_tac >- EVAL_TAC \\ disch_then (mp_tac o GSYM) \\ simp [get_var_mget_var] \\
  fs [relS_def, relS_var_def]);
 
+(* Could move this further up *)
+val computer_def = Define `
+ computer = MAP (intro_cvars cvars) [prog; prog_acc]`;
+
 val computer_Next_relM_run = Q.store_thm("computer_Next_relM_run",
  `!n fextv fext init vs.
   vars_has_type vs ag32types /\ relM init vs /\ relM_fextv fextv fext
   ==>
-  ?vs'. mrun fextv (MAP (intro_cvars cvars) [prog; prog_acc]) vs n = INR vs' /\
+  ?vs'. mrun fextv computer vs n = INR vs' /\
         relM (circuit addacc_next init fext n) vs'`,
  rpt strip_tac \\ match_mp_tac mstep_commit_mrun \\ qexists_tac `ag32types` \\ rpt conj_tac
  >- simp [circuit_def]
  >- simp []
  (* TODO: Not sure why match_mp_tac doesn't work here... *)
- \\ rpt strip_tac \\ drule_strip (SIMP_RULE (srw_ss()) [] computer_Next_relM) \\ simp []);
+ \\ rpt strip_tac \\ drule_strip (SIMP_RULE (srw_ss()) [] computer_Next_relM) \\ simp [computer_def]);
+
+(** Lift INIT_REL_circuit to Verilog level **)
+
+(* TODO: Move *)
+
+val mget_var_ALOOKUP = Q.store_thm("mget_var_ALOOKUP",
+ `!s name v. mget_var s name = INR v <=> ALOOKUP s name = SOME v`,
+ rw [mget_var_def] \\ CASE_TAC);
+
+val ver2w_def = Define `
+ ver2w v = sum_map v2w (ver2v v)`;
+
+val ver2w_w2ver = Q.store_thm("ver2w_w2ver",
+ `!v. ver2w (w2ver v) = INR v`,
+ simp [ver2w_def, w2ver_def, ver2v_def, sum_mapM_VBool, sum_map_def]);
+
+(* Similar to REL, but for initial state *)
+val INIT_verilog_def = Define `
+ INIT_verilog env <=>
+  (* Machine implementation registers *)
+  WORD (3w:word3) (THE (ALOOKUP env "state")) /\
+  BOOL F (THE (ALOOKUP env "acc_arg_ready")) /\
+  WORD (0w:word3) (THE (ALOOKUP env "command")) /\
+  WORD (5w:word3) (THE (ALOOKUP env "do_delay_write")) /\
+  BOOL F (THE (ALOOKUP env "do_interrupt")) /\
+  BOOL F (THE (ALOOKUP env "interrupt_req"))`;
+
+val INIT_fext_def = Define `
+ INIT_fext fext <=>
+ fext.io_events = [] /\
+ fext.ready /\
+ fext.interrupt_state = InterruptReady /\
+ ~fext.interrupt_ack`;
+
+val (var_has_type_tm, mk_var_has_type, dest_var_has_type, is_var_has_type) = syntax_fns3 "verilogType" "var_has_type";
+
+fun var_has_type_to_old_CONV tm =
+ if is_abs tm then
+   ABS_CONV var_has_type_to_old_CONV tm
+ else if is_var_has_type tm then let
+   val (_, _, ty) = dest_var_has_type tm
+ in
+   if is_VBool_t ty then (* BOOL *)
+     PURE_REWRITE_CONV [GSYM var_has_type_old_var_has_type_BOOL] tm
+   else if is_VArray_t ty then let
+     val is = dest_VArray_t ty
+     val len = length is
+   in
+     if len = 1 then (* WORD, TODO: assumes numerals in index position *) let
+       val dimindex_rw = is |> hd |> dest_numeral |> mk_numeric_type |> mk_dimindex |> EVAL |> SYM
+     in
+       PURE_REWRITE_CONV [dimindex_rw, GSYM var_has_type_old_var_has_type_WORD] tm
+     end else if len = 2 then (* WORD_ARRAY, TODO: does not work if index same... *) let
+       val dimword_rw = is |> hd |> dest_numeral |> Arbnumcore.log2 |> mk_numeric_type |> mk_dimword |> EVAL |> SYM
+       val dimindex_rw = is |> tl |> hd |> dest_numeral |> mk_numeric_type |> mk_dimindex |> EVAL |> SYM
+     in
+       PURE_REWRITE_CONV [dimword_rw, dimindex_rw, GSYM var_has_type_old_var_has_type_WORD_ARRAY] tm
+     end else
+       ALL_CONV tm
+   end else
+     ALL_CONV tm
+ end else if is_comb tm then
+   COMB_CONV var_has_type_to_old_CONV tm
+ else ALL_CONV tm;
+
+val relM_backwards = Q.store_thm("relM_backwards",
+ `!vs. vars_has_type vs relMtypes ==> ?hol_s. relM hol_s vs`,
+ simp [vars_has_type_def, relMtypes_def, relM_def, relM_var_def, mget_var_ALOOKUP] \\ rpt gen_tac \\
+
+ CONV_TAC var_has_type_to_old_CONV \\
+
+ simp [var_has_type_old_def, var_has_value_def] \\
+
+ disch_then (MAP_EVERY (REPEAT_TCL CHOOSE_THEN ASSUME_TAC) o CONJUNCTS) \\
+
+ (fn g as (asl, _) => let
+     val hol_s = foldr (fn (assm, acc) => let
+                          val (lconj, rconj) = dest_conj assm
+                          val name = lconj |> lhs |> rand |> fromHOLstring
+                          val update = lookup name updates
+                          val rep = rconj |> rator |> rand
+                        in
+                          mk_comb(mk_comb (update, (mk_K_1 (rep, type_of rep))), acc)
+                        end)
+                       ``ARB:state_circuit``
+                       asl
+  in
+    EXISTS_TAC hol_s g
+  end) \\
+
+ simp []);
+
+val INIT_backwards_mem_def = Define `
+ INIT_backwards_mem (mem : word32 -> word32) (i : word32) = (7 >< 0) (mem (align 2 i) >>>~ (8w * (1 >< 0) i))`;
+
+val align_addr_align = Q.prove(
+ `!w. align_addr w = align 2 w`,
+ rw [align_addr_def, align_def] \\ blastLib.BBLAST_TAC);
+
+val word4lt = WORD_DECIDE ``!(w:word32). w <+ 4w <=> w = 0w \/ w = 1w \/ w = 2w \/ w = 3w``;
+
+val align_align_2_4 = Q.prove(
+ `!w (addr:word32).
+   w <+ 4w ==> align 2 (align 2 addr + w) = align 2 addr`,
+ rpt strip_tac \\ fs [word4lt] \\ rveq \\
+ simp [align_def] \\ blastLib.BBLAST_TAC);
+
+val align_align_2_4_add = Q.prove(
+ `!w (addr:word32). w <+ 4w ==> (1 >< 0) (align 2 addr + w) = w`,
+ rpt strip_tac \\ fs [word4lt] \\ rveq \\
+ simp [align_def] \\ blastLib.BBLAST_TAC);
+
+val align_align_2_4_add_0 = align_align_2_4_add |> Q.SPEC `0w` |> SIMP_RULE (srw_ss()) [];
+
+val mem_eq_INIT_backwards_mem = Q.store_thm("mem_eq_INIT_backwards_mem",
+ `!memw. ∃memb. mem_eq memw memb`,
+ gen_tac \\ qexists_tac `INIT_backwards_mem memw` \\
+ rw [mem_eq_def, word_at_addr_def, INIT_backwards_mem_def, align_addr_align, align_align_2_4, align_align, align_align_2_4_add, align_align_2_4_add_0] \\
+ simp [align_def] \\ blastLib.BBLAST_PROVE_TAC);
+
+val INIT_backwards = Q.store_thm("INIT_backwards",
+ `!t fext env mem_start.
+   relM t env /\ INIT_verilog env /\ INIT_fext fext ==>
+   ?s mem.
+    INIT fext t (s with <| PC := mem_start + 64w;
+                           R := (0w =+ mem_start) s.R;
+                           MEM := mem;
+                           io_events := [] |>)`,
+ rw [relM_def, INIT_def, INIT_verilog_def, INIT_fext_def] \\
+
+ qexists_tac `<| R := t.R; CarryFlag := t.CarryFlag; OverflowFlag := t.OverflowFlag;
+                 data_in := t.data_in; data_out := t.data_out |>` \\
+ simp [INIT_R_def, combinTheory.UPDATE_APPLY] \\
+
+ qspec_then `fext.mem` strip_assume_tac mem_eq_INIT_backwards_mem \\ asm_exists_tac \\
+
+ rfs [relM_var_def, WORD_def, BOOL_def, mget_var_ALOOKUP, w2ver_bij]);
+
+val fext_accessor_verilog_def = Define `
+ fext_accessor_verilog =
+  <| get_command := \s. OUTR (ver2w (THE (ALOOKUP (OUTR s) "command")));
+     get_PC := \s. OUTR (ver2w (THE (ALOOKUP (OUTR s) "PC")));
+     get_data_addr := \s. OUTR (ver2w (THE (ALOOKUP (OUTR s) "data_addr")));
+     get_data_wdata := \s. OUTR (ver2w (THE (ALOOKUP (OUTR s) "data_wdata")));
+     get_data_wstrb := \s. OUTR (ver2w (THE (ALOOKUP (OUTR s) "data_wstrb")));
+
+     get_interrupt_req := \s. OUTR (ver2bool (THE (ALOOKUP (OUTR s) "interrupt_req"))) |>`;
+
+(* To cong thm here also? *)
+val is_interrupt_interface_verilog = Q.store_thm("is_interrupt_interface_verilog",
+ `!vs init fext fextv.
+   vars_has_type vs ag32types /\ relM init vs /\ relM_fextv fextv fext /\
+   is_interrupt_interface fext_accessor_verilog (mrun fextv computer vs) fext ==>
+   is_interrupt_interface fext_accessor_circuit (circuit addacc_next init fext) fext`,
+ simp [is_interrupt_interface_def, fext_accessor_circuit_def, fext_accessor_verilog_def] \\ rpt strip_tac \\
+
+ drule_strip computer_Next_relM_run \\ pop_assum (qspec_then `n` strip_assume_tac) \\
+
+ first_x_assum (qspec_then `n` assume_tac) \\
+ TOP_CASE_TAC \\ fs [] \\
+ rfs [relM_def, relM_var_def, mget_var_ALOOKUP, BOOL_def, ver2bool_def]);
+
+val is_mem_cong = Q.store_thm("is_mem_cong",
+ `!accessors1 step1 accessors2 step2 fext.
+   (!n. accessors1.get_command (step1 n) = accessors2.get_command (step2 n) /\
+        accessors1.get_PC (step1 n) = accessors2.get_PC (step2 n) /\
+        accessors1.get_data_addr (step1 n) = accessors2.get_data_addr (step2 n) /\
+        accessors1.get_data_wdata (step1 n) = accessors2.get_data_wdata (step2 n) /\
+        accessors1.get_data_wstrb (step1 n) = accessors2.get_data_wstrb (step2 n)) ==>
+   (is_mem accessors1 step1 fext <=> is_mem accessors2 step2 fext)`,
+ rw [is_mem_def, fext_accessor_circuit_def, fext_accessor_verilog_def]);
+
+val is_mem_cong' = is_mem_cong
+ |> SPEC_ALL
+ |> MATCH_MP (simpLib.SIMP_PROVE (srw_ss()) [] ``!a b c. (a ==> (b <=> c)) ==> (b ==> a ==> c)``)
+ |> GEN_ALL;
+
+val is_mem_verilog = Q.store_thm("is_mem_verilog",
+ `!vs init fext fextv.
+   vars_has_type vs ag32types /\ relM init vs /\ relM_fextv fextv fext /\
+   is_mem fext_accessor_verilog (mrun fextv computer vs) fext ==>
+   is_mem fext_accessor_circuit (circuit addacc_next init fext) fext`,
+ rpt strip_tac \\ pop_assum (fn th => match_mp_tac (MATCH_MP is_mem_cong' th)) \\ gen_tac \\
+
+ simp [fext_accessor_circuit_def, fext_accessor_verilog_def] \\
+
+ drule_strip computer_Next_relM_run \\
+ pop_assum (qspec_then `n` strip_assume_tac) \\
+ qpat_x_assum `relM init vs` kall_tac \\ (* just for cleanup *)
+
+ fs [relM_def, relM_var_def, mget_var_ALOOKUP, WORD_def, ver2w_w2ver]);
 
 val INIT_REL_circuit_verilog = Q.store_thm("INIT_REL_circuit_verilog",
-  `!n c s init fext fextv vs.
-   c = circuit addacc_next init fext /\
-   is_mem c fext /\
+  `!n init mem_start fext fextv vstep.
+   vstep = mrun fextv computer init /\
+
+   relM_fextv fextv fext /\
+   is_mem fext_accessor_verilog vstep fext /\
+   is_interrupt_interface fext_accessor_verilog vstep fext /\
+   is_mem_start_interface fext mem_start /\
+
    mem_no_errors fext /\
 
-   vars_has_type vs ag32types /\
-   relM init vs /\
-   relM_fextv fextv fext /\
+   vars_has_type init (relMtypes ++ ag32types) /\
+   INIT_verilog init /\
+   INIT_fext (fext 0) /\
 
-   INIT (fext 0) init s ==>
-   ?m vs' cvs'.
-    mrun fextv (MAP (intro_cvars cvars) [prog; prog_acc]) vs m = INR vs' /\
-    relM cvs' vs' /\
-    REL (fext m) cvs' (FUNPOW Next n s)`,
- simp [] \\ rpt strip_tac \\
+   (!s.
+    mem_eq (fext 0).mem s.MEM /\
+    s.io_events = [] /\
+    s.R 0w = mem_start /\
+    s.PC = mem_start + 64w ==>
+    (FUNPOW Next n s).io_events = [] (* <-- just an example property *))
+   ==>
+   ?m vs'.
+    vstep m = INR vs' /\
+    (fext m).io_events = []
+    (*LIST_REL mem_eq (fext m).io_events s'.io_events*)`,
+ simp [vars_has_type_append] \\ rpt strip_tac \\
 
- drule_strip (SIMP_RULE (srw_ss()) [] INIT_REL_circuit) \\
- disch_then (qspecl_then [`n`, `s`] mp_tac) \\
- impl_tac >- simp [is_acc_addacc] \\ strip_tac \\
+ drule_strip relM_backwards \\
+ drule_strip INIT_backwards \\
+ pop_assum (qspec_then `mem_start` strip_assume_tac) \\
 
- drule_strip computer_Next_relM_run \\ pop_assum (qspec_then `m` strip_assume_tac) \\ fs [] \\
- asm_exists_tac \\ simp [] \\ asm_exists_tac \\ simp []);
+ drule_strip is_interrupt_interface_verilog \\
+ qspecl_then [`hol_s`, `fext`] assume_tac is_acc_addacc \\
+ drule_strip is_mem_verilog \\
+
+ drule_strip (SIMP_RULE (srw_ss()) [] INIT_REL_circuit) \\ simp [combinTheory.UPDATE_APPLY] \\
+ disch_then (qspec_then `n` strip_assume_tac) \\
+
+ (* Step to REL-valid state *)
+ drule_strip (SIMP_RULE (srw_ss()) [circuit_0] circuit_0_next) \\
+ impl_tac >- fs [INIT_def] \\ strip_tac \\
+
+ drule_strip computer_Next_relM_run \\ pop_assum (qspec_then `m'` strip_assume_tac) \\
+ asm_exists_tac \\
+
+ qmatch_asmsub_abbrev_tac `INIT _ _ s'` \\
+ first_x_assum (qspec_then `s'` mp_tac) \\
+ qunabbrev_tac `s'` \\ simp [combinTheory.UPDATE_APPLY] \\
+
+ fs [REL_def, INIT_def] \\ metis_tac [LIST_REL_NIL]);
 
 val _ = export_theory ();
